Strata/DL/Imperative/HasVars.lean
@@ -19,10 +19,8 @@ class HasVarsPure (P : PureExpr) (α : Type) where
 /-! # Imperative Variable Lookup : HasVarsImp -/
 
 class HasVarsImp (P : PureExpr) (α : Type) where
-  definedVars : α → List P.Ident
+  definedVars : α → Bool/-exclude vars not visible from outside?-/ → List P.Ident
   modifiedVars : α → List P.Ident
-  modifiedOrDefinedVars : α → List P.Ident
-          := λ e ↦ definedVars e ++ modifiedVars e
 
 ---------------------------------------------------------------------
 
@@ -42,7 +40,6 @@ class HasVarsTrans
   definedVarsTrans : (String → Option PT) → α → List P.Ident
   modifiedVarsTrans : (String → Option PT) → α → List P.Ident
   getVarsTrans : (String → Option PT) → α → List P.Ident
-  modifiedOrDefinedVarsTrans : (String → Option PT) → α → List P.Ident
   allVarsTrans : (String → Option PT) → α → List P.Ident
   := λ π a ↦ modifiedVarsTrans π a ++ getVarsTrans π a
 
