Strata/Languages/Core/StatementSemanticsProps.lean
@@ -1760,27 +1760,6 @@ theorem EvalCmdDefMonotone' :
   | eval_set_nondet Hup Hwf => exact UpdateStateDefMonotone Hdef Hup
   | _ => exact Hdef
 
-theorem EvalCmdTouch
-  [HasVal P] [HasFvar P] [HasBool P] [HasBoolVal P] [HasNot P] :
-  EvalCmd P δ σ c σ' f →
-  TouchVars σ (HasVarsImp.modifiedOrDefinedVars c) σ' := by
-  intro Heval
-  induction Heval <;> simp [HasVarsImp.modifiedOrDefinedVars, Cmd.definedVars, Cmd.modifiedVars]
-  case eval_init x' δ σ x v σ' σ₀ e Hsm Hup Hwf =>
-    apply TouchVars.init_some Hup
-    constructor
-  case eval_init_unconstrained x' δ σ x v σ' σ₀ Hup Hwf =>
-    apply TouchVars.init_some Hup
-    constructor
-  case eval_set δ σ x v σ' σ₀ e Hsm Hup Hwf =>
-    exact TouchVars.update_some Hup TouchVars.none
-  case eval_set_nondet x v σ' σ₀ e Hsm Hup Hwf =>
-    exact TouchVars.update_some Hup TouchVars.none
-  case eval_assert_pass => exact TouchVars.none
-  case eval_assert_fail => exact TouchVars.none
-  case eval_assume => exact TouchVars.none
-  case eval_cover => exact TouchVars.none
-
 theorem UpdateStatesHavocVars : UpdateStates σ vars modvals σ' → HavocVars σ vars σ' := by
   intros H
   induction vars generalizing σ modvals
